ems/SimGlobalIndex2Explicit2.v
@@ -1,0 +1,61 @@
+Require Import Coqlib.
+Require Import ITreelib.
+Require Import Any.
+Require Import STS.
+Require Import Behavior.
+Require Import ModSem.
+Require Import Skeleton.
+Require Import Coq.Relations.Relation_Definitions.
+Require Import Relation_Operators.
+Require Import RelationPairs.
+From Ordinal Require Import Ordinal Arithmetic.
+From Ordinal Require Import ClassicalOrdinal.
+
+Require Import SimGlobalExplicit SimGlobalIndex2Explicit.
+
+Set Implicit Arguments.
+
+Section PROOF.
+
+  Lemma gen_exp2simg_exp
+        R0 R1 (RR: Ord.t -> Ord.t -> R0 -> R1 -> Prop)
+        (itr_src: itree eventE R0)
+        (itr_tgt: itree eventE R1)
+        (f_src f_tgt: Ord.t)
+        (g_src g_tgt: Ord.t)
+        (GEN: gen_exp RR f_src f_tgt (g_src) (itr_src) (g_tgt) (itr_tgt))
+    :
+    simg_exp RR (f_tgt + g_src)%ord (f_src + g_tgt)%ord itr_src itr_tgt.
+  Proof.
+    ginit.
+    revert_until RR.
+    gcofix CIH. i. move f_src before CIH. revert_until f_src.
+    pattern f_src. revert f_src. eapply (well_founded_induction Ord.lt_well_founded).
+    intros f_src IHo. i. induction GEN.
+    { gstep. econs 1. admit "RR". }
+    { gstep. econs 2. i. specialize (GEN x_src x_tgt EQ). gfinal. left. eauto. }
+    { gstep. econs 3. instantiate (1:= (f_tgt + g_src0)%ord). apply OrdArith.lt_add_r. auto.
+      gfinal. left. eauto. }
+    { gstep. econs 4. instantiate (1:= (f_src + g_tgt0)%ord). apply OrdArith.lt_add_r. auto.
+      gfinal. left. eauto. }
+    { gstep. econs 5. instantiate (1:= (f_tgt + g_src0)%ord). apply OrdArith.lt_add_r. auto.
+      des. exists x. gfinal. left. eauto. }
+    { gstep. econs 6. instantiate (1:= (f_src + g_tgt0)%ord). apply OrdArith.lt_add_r. auto.
+      i. gfinal. left. eauto. }
+    { gstep. econs 7. instantiate (1:= (f_tgt + g_src0)%ord). apply OrdArith.lt_add_r. auto.
+      i. gfinal. left. eauto. }
+    { gstep. econs 8. instantiate (1:= (f_src + g_tgt0)%ord). apply OrdArith.lt_add_r. auto.
+      des. exists x. gfinal. left. eauto. }
+    { assert (TODO: simg_aux RR f_src0 f_tgt0 itr_src itr_tgt ->
+                    exists gs gt, gen_exp RR f_src0 f_tgt0 gs itr_src gt itr_tgt).
+      { admit "TODO". }
+      apply TODO in SIM. des. guclo simg_exp_leC_spec. econs.
+      { admit "RR?". }
+      3:{ eapply IHo. 2: eauto. auto. }
+      { admit "needs lex-order". }
+      { admit "needs lex-order". }
+
+  Abort.
+
+
+End PROOF.
